splat-mon.sml
@@ -1,11 +1,11 @@
 (*---------------------------------------------------------------------------*)
 (* Maps from Json representation of AADL to AST and then to HOL. Solely      *)
-(* aimed at extracting filter properties, plus support definitions.          *)
+(* aimed at extracting monitor properties, plus support definitions.          *)
 (*---------------------------------------------------------------------------*)
 
 open Lib Feedback HolKernel boolLib MiscLib bossLib;
 
-local open AADL ptltlSyntax regexpLib regexpSyntax in end
+local open AADL ptltlSyntax regexpLib regexpSyntax realLib realSyntax in end
 
 val ERR = Feedback.mk_HOL_ERR "splat-mon";
 
@@ -67,8 +67,11 @@ fun synthesize_monitor monitor =
    monitor_data monitor
  end
 
+val args = ["examples/UAS.json"];
 
 (*
+HAMR::Bit_Codec_Max_Size: It is attached to the types declared for the channel.
+
 val args = ["examples_monitor/req_resp_monitor.json"];
 val args = ["examples_monitor/geo_monitor.json"];
 val args = ["examples_monitor/Coord-Mon.json"];
@@ -80,6 +83,16 @@ val args = ["examples_monitor/RunTimeMonitor_Simple_Example_V1.json"];
 val args = ["examples_monitor/Datacentric_monitor.json"];
 *)
 
+fun extract_filter (pkgName,(tydecs,fndecs,filtdecs,mondecs)) = filtdecs;
+
+fun extract_consts ("CM_Property_Set",(tydecs,fndecs,filtdecs,mondecs)) =
+     let open AADL
+         fun dest_const_dec (ConstDec ((_,cname),ty,i)) = (cname,i)
+     in mapfilter dest_const_dec fndecs
+     end
+  | extract_consts otherwise = raise ERR "extract_consts" "looking for package CM_Property_Set"
+
+
 fun main () =
  let val _ = stdErr_print "splat-mon: \n"
      val args = CommandLine.arguments()
@@ -88,10 +101,15 @@ fun main () =
 	   ("Parsing "^jsonfile^" ... ") "succeeded.\n"
      val pkgs = apply_with_chatter AADL.scrape_pkgs jpkg
                   "Converting Json to AST ... " "succeeded.\n"
+     val filter_decs = List.concat (map extract_filter pkgs)
+     val const_alist = tryfind extract_consts pkgs
+     val filter_CakeML_files = map (AADL.inst_filter_template "." const_alist) filter_decs
      val thyName = fst (last pkgs)
      val _ = new_theory thyName
      val logic_defs = apply_with_chatter (AADL.pkgs2hol thyName) pkgs
 	   "Converting AST to logic ...\n" "---> succeeded.\n"
+     val filters = #4 logic_defs
+     val filter_thms = []
      val monitors = #5 logic_defs
      val monitor_thms = apply_with_chatter (List.map synthesize_monitor) monitors
 	   "Synthesizing monitors ...\n" "---> succeeded.\n"
